emma_orig.v
@@ -6,6 +6,7 @@ Import FormulaMultiSet. (* and this *)
 Open Scope ILL_scope.
 
 (* Declaration of basic propositions. *)
+Declare Scope Emma.
 Notation "'P'" := (Proposition 1%nat):Emma.
 Notation "'R'" := (Proposition 2%nat):Emma. (* Meets Rodolph *)
 Notation "'G'" := (Proposition 3%nat):Emma.
@@ -23,17 +24,17 @@ Open Scope Emma.
 Lemma simpl_ex: {P ⊸ M, P, !(S ⊸ A)} ⊢ A ⊕ M.
 Proof with try solve [ apply Id;reflexivity | prove_multiset_eq].
   bang_w (S ⊸ A)...
-  weak_impl_l (P) (M)...
+  weak_impl_l P M...
   apply Oplus_R_2...
 Defined.
 
 (* EXAMPLE OF IMPOSSIBLE INTERNAL CHOICE *)
-Lemma originelle :              
+Lemma originelle :
   {P&1, R, G, B&1, !(S⊸A), (E⊸A)&1, (P⊸M)&1,(R⊸1)&(R⊸E), (G⊸1)⊕(G⊸S), 1⊕((B⊸S)&(B⊸1))  } ⊢ A ⊕ M .
 Proof with try solve [ apply Id;reflexivity | prove_multiset_eq].
   and_l_2 (R⊸1) (R⊸E).
   oplus_l (G ⊸ 1) (G ⊸ S).
-  Focus 2.
+  2:{
   weak_impl_l G S...
   weak_impl_l R E...
   bang_c (S ⊸ A).
@@ -43,67 +44,67 @@ Proof with try solve [ apply Id;reflexivity | prove_multiset_eq].
   weak_impl_l E A... (* THERE ARE TWO A *)
 Abort.
 
-Lemma originelle :              
+Lemma originelle :
   {P&1, R, G, B&1, !(S⊸A), (E⊸A)&1, (P⊸M)&1,(R⊸1)&(R⊸E), (G⊸1)⊕(G⊸S), 1⊕((B⊸S)&(B⊸1))  } ⊢ A ⊕ M .
 Proof with try solve [ apply Id;reflexivity | prove_multiset_eq].
   oplus_l (G ⊸ 1) (G ⊸ S).
   - (* Left branch *)
-    weak_impl_l (G) 1...
+    weak_impl_l G 1...
     one_l.
     oplus_l 1 ((B ⊸ S) & (B ⊸ 1)).
-    all:swap 1 2. (* switch subgoals to match the order of the document *)
+    all: swap 1 2. (* switch subgoals to match the order of the document *)
     (* Left left. *) 
     + and_l_2 (B ⊸ S) (B ⊸ 1).
-      and_l_1  (B) 1.
-      weak_impl_l (B) 1...
-      one_l.  
+      and_l_1 B 1.
+      weak_impl_l B 1...
+      one_l.
       and_l_1 (R ⊸ 1) (R ⊸ E).
-      weak_impl_l (R) 1...
-      and_l_1 (P) 1.
+      weak_impl_l R 1...
+      and_l_1 P 1.
       and_l_2 (E ⊸ A) 1.
       and_l_1 (P ⊸ M) 1.
       do 2 one_l.
       bang_w (S ⊸ A)...
-      weak_impl_l (P) (M)...
+      weak_impl_l P M...
       apply Oplus_R_2...
     + (* Left right *)
-      and_l_2 (B) 1.
+      and_l_2 B 1.
       do 2 one_l.
-      and_l_2 (P) 1.
+      and_l_2 P 1.
       and_l_1 (E ⊸ A) 1.
       and_l_2 (P ⊸ M) 1.
       and_l_2 (R ⊸ 1) (R ⊸ E).
       do 2 one_l.
       bang_w (S ⊸ A)...
-      weak_impl_l (R) (E)...
-      weak_impl_l (E) (A)...
+      weak_impl_l R E...
+      weak_impl_l E A...
       apply Oplus_R_1...
   - (* Right branch of the document *)
-    weak_impl_l (G) (S)...
+    weak_impl_l G S...
     and_l_1(R ⊸ 1) (R ⊸ E).
-    weak_impl_l (R) 1...
+    weak_impl_l R 1...
     one_l. (* +L in the document but actually 1L *)
     oplus_l 1 ((B ⊸ S) & (B ⊸ 1)).
     + (* Right left *)
-      and_l_2 (P) 1.
-      and_l_2 (B) 1.
+      and_l_2 P 1.
+      and_l_2 B 1.
       and_l_2 (E ⊸ A)  1.
-      and_l_2 (P ⊸ M) 1.  
-      repeat one_l. 
+      and_l_2 (P ⊸ M) 1.
+      repeat one_l.
       bang_d (S ⊸ A)... (* !D instead of WL *)
-      weak_impl_l (S) (A)...
+      weak_impl_l S A...
       apply Oplus_R_1...
     + (* Right right *)
       and_l_2 (B ⊸ S) (B ⊸ 1).
-      and_l_1 (B) 1.
-      weak_impl_l (B) 1...
+      and_l_1 B 1.
+      weak_impl_l B 1...
       one_l.
-      and_l_2 (P) 1.
+      and_l_2 P 1.
       and_l_2 (E ⊸ A) 1.
       and_l_2 (P ⊸ M) 1.
       repeat one_l.
       bang_d (S ⊸ A)... (* !D instead of WL *)
-      weak_impl_l (S) (A)...
+      weak_impl_l S A...
       apply Oplus_R_1...
 Defined.
 
@@ -151,40 +152,40 @@ Ltac search_goal n g :=
       apply Oplus_R_2;search_goal m g
     end
   end.
-  
 
-Lemma originelle' :              
+
+Lemma originelle' :
   {P&1, R, G, B&1, !(S⊸A), (E⊸A)&1, (P⊸M)&1,(R⊸1)&(R⊸E), (G⊸1)⊕(G⊸S), 1⊕((B⊸S)&(B⊸1))  } ⊢ A ⊕ M .
 Proof with try solve [ apply Id;reflexivity | prove_multiset_eq].
   oplus_l (G ⊸ 1) (G ⊸ S).
-  - weak_impl_l (G) 1...
+  - weak_impl_l G 1...
     one_l.
     oplus_l 1 ((B ⊸ S) & (B ⊸ 1)).
-    + and_l_2 (B) 1.
+    + and_l_2 B 1.
       do 2 one_l.
-      and_l_2 (P) 1.
+      and_l_2 P 1.
       and_l_1 (E ⊸ A) 1.
       Time search_goal 6 ({R ⊸ E, E ⊸ A, R} ⊢ A ⊕ M).
       finish_proof_strong.
     + and_l_2 (B ⊸ S) (B ⊸ 1).
-      and_l_1  (B) 1.
-      weak_impl_l (B) 1...
+      and_l_1 B 1.
+      weak_impl_l B 1...
       one_l.  
       and_l_1 (R ⊸ 1) (R ⊸ E).
-      weak_impl_l (R) 1...
-      and_l_1 (P) 1.
+      weak_impl_l R 1...
+      and_l_1 P 1.
       Time search_goal 6 ({P ⊸ M, P} ⊢ A ⊕ M).
       finish_proof_strong.
-  - weak_impl_l (G) (S)...
+  - weak_impl_l G S...
     and_l_1(R ⊸ 1) (R ⊸ E).
-    weak_impl_l (R) 1...
+    weak_impl_l R 1...
     one_l.
     oplus_l 1 ((B ⊸ S) & (B ⊸ 1)).
     + search_goal 10 ({S, !(S ⊸ A)} ⊢ A ⊕ M).
       bang_d (S ⊸ A)... (* !D instead of WL *)
       finish_proof_strong.
     + and_l_2 (B ⊸ S) (B ⊸ 1).
-      and_l_1 (B) 1.
+      and_l_1 B 1.
       Time search_goal 10 ({S, !(S ⊸ A)} ⊢ A ⊕ M).
       bang_d (S ⊸ A)... (* !D instead of WL *)
       finish_proof_strong.
@@ -192,8 +193,8 @@ Proof with try solve [ apply Id;reflexivity | prove_multiset_eq].
 
 
 (*
-Lemma originelle2 :              
+Lemma originelle2 :
   {P&1, R, G, B&1, !(S⊸A), (E⊸A)&1, (P⊸M)&1,(R⊸1)&(R⊸E), (G⊸1)⊕(G⊸S), 1⊕((B⊸S)&(B⊸1))  } ⊢ A ⊕ M .
 
   and_l_2 (R⊸1) (R⊸E).
-*)  
+*)
