multiset.v
@@ -1,8 +1,9 @@
-Require Import Utf8_core Omega.
+Require Import Utf8_core Lia.
 Require Import FMapInterface.
 Require Import FMapFacts.
 Require Import FMapAVL.
 Require Import OrderedType.
+Require Import FunInd.
 Require Import multiset_spec.
 Module PreMake(X:OrderedType)(Maps:FMapInterface.S with Module E:=X) <: S(X).
   Module MapsFact := WFacts(Maps).
@@ -19,15 +20,14 @@ Module PreMake(X:OrderedType)(Maps:FMapInterface.S with Module E:=X) <: S(X).
     match Maps.find a ms with 
       | Some v => Maps.add a (S (plus n v)) ms
       | None => Maps.add a n ms
-    end 
-    . 
+    end.
 
   Fixpoint iter (B:Type) (f:A -> B -> B) (k:A) (v:nat) (acc:B) {struct v} : B := 
     match v with 
       | 0 => f k acc
       | S n => f k (iter B f k n acc)
     end.
-    
+
   Definition fold (B:Type) (f:A -> B -> B) ms v0 := 
     Maps.fold (iter B f) ms v0.
 
@@ -68,7 +68,7 @@ Module PreMake(X:OrderedType)(Maps:FMapInterface.S with Module E:=X) <: S(X).
 
   Definition eq_trans : forall ms1 ms2 ms3, eq ms1 ms2 -> eq ms2 ms3 -> eq ms1 ms3 := @MapsFact.Equal_trans nat.
 
-  Lemma add_morph_eq : forall a a', X.eq a a' -> forall ms ms',  eq ms ms' -> eq (add a ms) (add a' ms'). 
+  Lemma add_morph_eq : forall a a', X.eq a a' -> forall ms ms',  eq ms ms' -> eq (add a ms) (add a' ms').
   Proof.
     intros a a' H ms ms' H0.
     unfold eq,add in *.
@@ -83,7 +83,7 @@ Module PreMake(X:OrderedType)(Maps:FMapInterface.S with Module E:=X) <: S(X).
     reflexivity.
   Qed.
 
-  Definition union : t -> t -> t := fun ms1 ms2 => 
+  Definition union : t -> t -> t := fun ms1 ms2 =>
     Maps.fold add_multiple ms1 ms2.
 
   Module MapsPtes := FMapFacts.Properties(Maps).
@@ -97,7 +97,7 @@ Module PreMake(X:OrderedType)(Maps:FMapInterface.S with Module E:=X) <: S(X).
     destruct (Maps.find y y1); rewrite H; rewrite H0;reflexivity.
   Qed.
 
-  Lemma add_comm_aux : 
+  Lemma add_comm_aux :
     forall (B : Type)
       (k : A)
       (k' : A)
@@ -155,7 +155,7 @@ Module PreMake(X:OrderedType)(Maps:FMapInterface.S with Module E:=X) <: S(X).
     symmetry in abs.
     elim alpha_eq_k'.
     assumption.
-    intros abs. 
+    intros abs.
     symmetry in abs.
     elim alpha_eq_k.
     assumption.
@@ -172,48 +172,46 @@ Module PreMake(X:OrderedType)(Maps:FMapInterface.S with Module E:=X) <: S(X).
     split;intros H1.
     apply add_comm_aux;assumption.
     apply add_comm_aux;try assumption.
-    intros abs. 
+    intros abs.
     symmetry in abs.
     elim H.
     assumption.
   Qed.
-  
+
   Lemma transpose_neqkey_equal_add_multiple : MapsPtes.transpose_neqkey Maps.Equal add_multiple.
   Proof.
     red.
     intros k k' e e' a H.
     unfold add_multiple.
     case_eq (Maps.find k' a);case_eq (Maps.find k a).
-    {
-      intros n2 Heq2.
+    - intros n2 Heq2.
       intros n1 Heq1.
       rewrite MapsPtes.F.add_neq_o;[ | intro abs;elim H;symmetry;assumption ].
       rewrite MapsPtes.F.add_neq_o;[ | assumption].
       rewrite Heq1;rewrite Heq2.
       apply add_comm'.
       assumption.
-    }
-    { intros Heq2.
+    - intros Heq2.
       intros n1 Heq1.
       rewrite MapsPtes.F.add_neq_o;[ | intro abs;elim H;symmetry;assumption ].
       rewrite MapsPtes.F.add_neq_o;[ | assumption].
       rewrite Heq1;rewrite Heq2.
       apply add_comm'.
-      assumption. }
-    { intros n2 Heq2.
+      assumption.
+    - intros n2 Heq2.
       intros Heq1.
       rewrite MapsPtes.F.add_neq_o;[ | intro abs;elim H;symmetry;assumption ].
       rewrite MapsPtes.F.add_neq_o;[ | assumption].
       rewrite Heq1;rewrite Heq2.
       apply add_comm'.
-      assumption. }
-    { intros Heq2.
+      assumption.
+    - intros Heq2.
       intros Heq1.
       rewrite MapsPtes.F.add_neq_o;[ | intro abs;elim H;symmetry;assumption ].
       rewrite MapsPtes.F.add_neq_o;[ | assumption].
       rewrite Heq1;rewrite Heq2.
       apply add_comm'.
-      assumption. }
+      assumption.
   Qed.
 
 
@@ -224,41 +222,38 @@ Module PreMake(X:OrderedType)(Maps:FMapInterface.S with Module E:=X) <: S(X).
     unfold union,eq.
     pattern a,(Maps.fold add_multiple a ms).
     apply MapsPtes.fold_rec_bis.
-
-    { intros m m' a0 H H0 a' H1 ms' H2.
+    - intros m m' a0 H H0 a' H1 ms' H2.
       apply H0.
-      rewrite H;exact H1.
-      assumption. }
-
-    { intros a' H ms' H0.
+      + rewrite H;exact H1.
+      + assumption.
+    - intros a' H ms' H0.
       rewrite MapsPtes.fold_Empty.
-      assumption.
-      auto with *.
-      clear -H.
-      unfold Maps.Equal, Maps.Empty in *.
-      intros a e.
-      intros abs.
-      rewrite MapsPtes.F.find_mapsto_iff in abs.
-      generalize (H a).
-      rewrite abs.
-      rewrite MapsPtes.F.empty_o.
-      discriminate. }
-
-    { intros k e a0 m' H H0 H1 a' H2 ms' H3.
+      + assumption.
+      + auto with *.
+      + clear -H.
+        unfold Maps.Equal, Maps.Empty in *.
+        intros a e.
+        intros abs.
+        rewrite MapsPtes.F.find_mapsto_iff in abs.
+        generalize (H a).
+        rewrite abs.
+        rewrite MapsPtes.F.empty_o.
+        discriminate.
+    - intros k e a0 m' H H0 H1 a' H2 ms' H3.
       rewrite <- MapsPtes.fold_Equal.
-      5:eexact H2.
-      rewrite MapsPtes.fold_add.
-      rewrite H1.
-      reflexivity.
-      reflexivity.
-      assumption.
-      auto with *.
-      apply add_multiple_morph_Proper.
-      apply transpose_neqkey_equal_add_multiple.
-      apply H0.
-      auto with *.
-      apply add_multiple_morph_Proper.
-      apply transpose_neqkey_equal_add_multiple. }
+      5:{ eexact H2. }
+      + rewrite MapsPtes.fold_add.
+        * rewrite H1.
+          -- reflexivity.
+          -- reflexivity.
+          -- assumption.
+        * auto with *.
+        * apply add_multiple_morph_Proper.
+        * apply transpose_neqkey_equal_add_multiple.
+        * apply H0.
+      + auto with *.
+      + apply add_multiple_morph_Proper.
+      + apply transpose_neqkey_equal_add_multiple.
   Qed.
 
   Lemma is_empty_empty : is_empty empty = true.
@@ -266,10 +261,10 @@ Module PreMake(X:OrderedType)(Maps:FMapInterface.S with Module E:=X) <: S(X).
     unfold is_empty,empty.
     rewrite <- MapsPtes.F.is_empty_iff.
     apply Maps.empty_1.
-  Qed.  
+  Qed.
 
 
-  Lemma is_empty_no_mem : forall ms, is_empty ms = true <-> (forall a, mem a ms = false). 
+  Lemma is_empty_no_mem : forall ms, is_empty ms = true <-> (forall a, mem a ms = false).
   Proof.
     intros ms.
     unfold is_empty,mem.
@@ -298,7 +293,7 @@ Module PreMake(X:OrderedType)(Maps:FMapInterface.S with Module E:=X) <: S(X).
     intros abs;unfold Maps.Empty in abs.
     apply (abs a (S n)).
     rewrite MapsPtes.F.add_mapsto_iff.
-    left;auto.
+    now left.
     rewrite MapsPtes.F.is_empty_iff in H.
     destruct (Maps.is_empty (Maps.add a (S n) ms)).
     elim H;reflexivity.
@@ -307,7 +302,7 @@ Module PreMake(X:OrderedType)(Maps:FMapInterface.S with Module E:=X) <: S(X).
     intros abs;unfold Maps.Empty in abs.
     apply (abs a 0).
     rewrite MapsPtes.F.add_mapsto_iff.
-    left;auto.
+    now left.
     rewrite MapsPtes.F.is_empty_iff in H.
     destruct (Maps.is_empty (Maps.add a 0 ms)).
     elim H;reflexivity.
@@ -318,19 +313,19 @@ Module PreMake(X:OrderedType)(Maps:FMapInterface.S with Module E:=X) <: S(X).
   Proof.
     unfold mem,add,add_multiple.
     intros a b ms Heq.
-    destruct (Maps.find b ms);  apply MapsPtes.F.add_eq_b;symmetry;assumption. 
+    now destruct (Maps.find b ms); apply MapsPtes.F.add_eq_b.
   Qed.
 
   Lemma mem_destruct : forall a b ms, mem a (add b ms) = true -> X.eq a b \/ mem a ms = true.
   Proof.
     intros a b ms.
     case (X.eq_dec a b).
-    auto.
-    unfold mem,add,add_multiple.
-    intros neq.    
-    destruct (Maps.find b ms);    rewrite MapsPtes.F.add_neq_b;auto.
+    - auto.
+    - unfold mem,add,add_multiple.
+      intros neq.
+      destruct (Maps.find b ms); rewrite MapsPtes.F.add_neq_b by intuition; auto.
   Qed.
-  
+
   Lemma mem_add_is_mem : forall a b ms, mem a ms = true -> mem a (add b ms) = true.
   Proof.
     intros a b ms.
@@ -339,129 +334,127 @@ Module PreMake(X:OrderedType)(Maps:FMapInterface.S with Module E:=X) <: S(X).
     apply add_is_mem;assumption.
     unfold mem,add,add_multiple.
     intros n H.
-    destruct (Maps.find b ms); rewrite MapsPtes.F.add_neq_b;auto.    
+    now destruct (Maps.find b ms); rewrite MapsPtes.F.add_neq_b by intuition.
   Qed.
 
-  Lemma add_multiple_comm : 
-    forall a v1 b v2 ms, 
-      eq 
-      (add_multiple a v1 (add_multiple b v2 ms)) 
+  Lemma add_multiple_comm :
+    forall a v1 b v2 ms,
+      eq
+      (add_multiple a v1 (add_multiple b v2 ms))
       (add_multiple b v2 (add_multiple a v1 ms)).
   Proof.
     unfold eq,add_multiple.
     intros a v1 b v2 ms.
     case (X.eq_dec a b);intros a_eq_b.
-    rewrite a_eq_b.
-
-    { case_eq (Maps.find b ms);[intro n1 |];intro Heq1.
-      rewrite MapsPtes.F.add_eq_o;[ | reflexivity].
-      rewrite a_eq_b.
-      rewrite MapsPtes.F.add_eq_o;[ | reflexivity].
-      rewrite a_eq_b.
-      rewrite Heq1.
-      rewrite a_eq_b.
-      intros k.
-      case (X.eq_dec k b);intros Heq2.
-      rewrite Heq2.
-      rewrite MapsPtes.F.add_eq_o.
-      rewrite MapsPtes.F.add_eq_o.
-      f_equal;omega.
-      reflexivity.
-      reflexivity.
-      do 4 (rewrite MapsPtes.F.add_neq_o;[|intros abs;elim Heq2;rewrite abs;reflexivity]).
-      reflexivity.
-      rewrite a_eq_b.
-      rewrite MapsPtes.F.add_eq_o.
-      rewrite MapsPtes.F.add_eq_o.
-      rewrite a_eq_b.
-      rewrite Heq1.
-      rewrite a_eq_b.
-      intro k.
-      case (X.eq_dec k b);intros Heq2.
-      rewrite Heq2.
-      rewrite MapsPtes.F.add_eq_o.
-      rewrite MapsPtes.F.add_eq_o.
-      f_equal; omega.
-      reflexivity.
-      reflexivity.
-      do 4 (rewrite MapsPtes.F.add_neq_o;[|intros abs;elim Heq2;rewrite abs;reflexivity]).
-      reflexivity.
-      reflexivity.
-      reflexivity. }
-
-    { case_eq (Maps.find b ms);[intro n1 |];intro Heq1.
-      rewrite MapsPtes.F.add_neq_o;[ | intros abs;elim a_eq_b;rewrite abs;reflexivity].
+    - rewrite a_eq_b.
+      case_eq (Maps.find b ms);[intro n1 |];intro Heq1.
+      + rewrite MapsPtes.F.add_eq_o;[ | reflexivity].
+        rewrite a_eq_b.
+        rewrite MapsPtes.F.add_eq_o;[ | reflexivity].
+        rewrite a_eq_b.
+        rewrite Heq1.
+        rewrite a_eq_b.
+        intros k.
+        case (X.eq_dec k b);intros Heq2.
+        * rewrite Heq2.
+          rewrite MapsPtes.F.add_eq_o.
+          -- rewrite MapsPtes.F.add_eq_o.
+             ++ f_equal;lia.
+             ++ reflexivity.
+          -- reflexivity.
+        * do 4 (rewrite MapsPtes.F.add_neq_o;[|intros abs;elim Heq2;rewrite abs;reflexivity]).
+          reflexivity.
+      + rewrite a_eq_b.
+        rewrite MapsPtes.F.add_eq_o.
+        * rewrite MapsPtes.F.add_eq_o.
+          -- rewrite a_eq_b.
+             rewrite Heq1.
+             rewrite a_eq_b.
+             intro k.
+             case (X.eq_dec k b);intros Heq2.
+             ++ rewrite Heq2.
+                rewrite MapsPtes.F.add_eq_o.
+                ** rewrite MapsPtes.F.add_eq_o.
+                   --- f_equal; lia.
+                   --- reflexivity.
+                ** reflexivity.
+             ++ do 4 (rewrite MapsPtes.F.add_neq_o;[|intros abs;elim Heq2;rewrite abs;reflexivity]).
+                reflexivity.
+          -- reflexivity.
+        * reflexivity.
+    - case_eq (Maps.find b ms);[intro n1 |];intro Heq1.
+      + rewrite MapsPtes.F.add_neq_o;[ | intros abs;elim a_eq_b;rewrite abs;reflexivity].
+        case_eq (Maps.find a ms);[intro n2 |];intro Heq2.
+        * rewrite MapsPtes.F.add_neq_o;[ | intros abs;elim a_eq_b;rewrite abs;reflexivity].
+          rewrite Heq1.
+          intros k.
+          case(X.eq_dec k a);intros Heq3.
+          -- rewrite Heq3.
+             rewrite MapsPtes.F.add_eq_o;[ | reflexivity].
+             rewrite MapsPtes.F.add_neq_o;[ | intros abs;elim a_eq_b;rewrite abs;reflexivity].
+             rewrite MapsPtes.F.add_eq_o;[ | reflexivity].
+             reflexivity.
+          -- rewrite MapsPtes.F.add_neq_o;[ | intros abs;elim Heq3;rewrite abs;reflexivity].
+             case(X.eq_dec k b);intros Heq4.
+             ++ rewrite Heq4.
+                repeat (rewrite MapsPtes.F.add_eq_o;[ | reflexivity]).
+                reflexivity.
+             ++ do 2 (rewrite MapsPtes.F.add_neq_o;[ | intros abs;elim Heq4;rewrite abs;reflexivity]).
+                rewrite MapsPtes.F.add_neq_o;[ | intros abs;elim Heq3;rewrite abs;reflexivity].
+                reflexivity.
+        * rewrite MapsPtes.F.add_neq_o;[ | intros abs;elim a_eq_b;rewrite abs;reflexivity].
+          rewrite Heq1.
+          intro k.
+          case(X.eq_dec k a);intros Heq3.
+          -- rewrite Heq3.
+             rewrite MapsPtes.F.add_eq_o;[ | reflexivity].
+             rewrite MapsPtes.F.add_neq_o;[ | intros abs;elim a_eq_b;rewrite abs;reflexivity].
+             rewrite MapsPtes.F.add_eq_o;[ | reflexivity].
+             reflexivity.
+          -- rewrite MapsPtes.F.add_neq_o;[ | intros abs;elim Heq3;rewrite abs;reflexivity].
+             case(X.eq_dec k b);intros Heq4.
+             ++ rewrite Heq4.
+                repeat (rewrite MapsPtes.F.add_eq_o;[ | reflexivity]).
+                reflexivity.
+             ++ do 2 (rewrite MapsPtes.F.add_neq_o;[ | intros abs;elim Heq4;rewrite abs;reflexivity]).
+                rewrite MapsPtes.F.add_neq_o;[ | intros abs;elim Heq3;rewrite abs;reflexivity].
+                reflexivity.
+    + rewrite MapsPtes.F.add_neq_o;[ | intros abs;elim a_eq_b;rewrite abs;reflexivity].
       case_eq (Maps.find a ms);[intro n2 |];intro Heq2.
-      rewrite MapsPtes.F.add_neq_o;[ | intros abs;elim a_eq_b;rewrite abs;reflexivity].
-      rewrite Heq1.
-      intros k.
-      case(X.eq_dec k a);intros Heq3.
-      rewrite Heq3.
-      rewrite MapsPtes.F.add_eq_o;[ | reflexivity].
-      rewrite MapsPtes.F.add_neq_o;[ | intros abs;elim a_eq_b;rewrite abs;reflexivity].
-      rewrite MapsPtes.F.add_eq_o;[ | reflexivity].
-      reflexivity.
-      rewrite MapsPtes.F.add_neq_o;[ | intros abs;elim Heq3;rewrite abs;reflexivity].
-      case(X.eq_dec k b);intros Heq4.
-      rewrite Heq4.
-      repeat (rewrite MapsPtes.F.add_eq_o;[ | reflexivity]).
-      reflexivity.
-      do 2 (rewrite MapsPtes.F.add_neq_o;[ | intros abs;elim Heq4;rewrite abs;reflexivity]).
-      rewrite MapsPtes.F.add_neq_o;[ | intros abs;elim Heq3;rewrite abs;reflexivity].
-      reflexivity.
-      rewrite MapsPtes.F.add_neq_o;[ | intros abs;elim a_eq_b;rewrite abs;reflexivity].
-      rewrite Heq1.
-      intro k.
-      case(X.eq_dec k a);intros Heq3.
-      rewrite Heq3.
-      rewrite MapsPtes.F.add_eq_o;[ | reflexivity].
-      rewrite MapsPtes.F.add_neq_o;[ | intros abs;elim a_eq_b;rewrite abs;reflexivity].
-      rewrite MapsPtes.F.add_eq_o;[ | reflexivity].
-      reflexivity.
-      rewrite MapsPtes.F.add_neq_o;[ | intros abs;elim Heq3;rewrite abs;reflexivity].
-      case(X.eq_dec k b);intros Heq4.
-      rewrite Heq4.
-      repeat (rewrite MapsPtes.F.add_eq_o;[ | reflexivity]).
-      reflexivity.
-      do 2 (rewrite MapsPtes.F.add_neq_o;[ | intros abs;elim Heq4;rewrite abs;reflexivity]).
-      rewrite MapsPtes.F.add_neq_o;[ | intros abs;elim Heq3;rewrite abs;reflexivity].
-      reflexivity.
-      rewrite MapsPtes.F.add_neq_o;[ | intros abs;elim a_eq_b;rewrite abs;reflexivity].
-      case_eq (Maps.find a ms);[intro n2 |];intro Heq2.
-      rewrite MapsPtes.F.add_neq_o;[ | intros abs;elim a_eq_b;rewrite abs;reflexivity].
-      rewrite Heq1.
-      intro k.
-      case(X.eq_dec k a);intros Heq3.
-      rewrite Heq3.
-      rewrite MapsPtes.F.add_eq_o;[ | reflexivity].
-      rewrite MapsPtes.F.add_neq_o;[ | intros abs;elim a_eq_b;rewrite abs;reflexivity].
-      rewrite MapsPtes.F.add_eq_o;[ | reflexivity].
-      reflexivity.
-      rewrite MapsPtes.F.add_neq_o;[ | intros abs;elim Heq3;rewrite abs;reflexivity].
-      case(X.eq_dec k b);intros Heq4.
-      rewrite Heq4.
-      repeat (rewrite MapsPtes.F.add_eq_o;[ | reflexivity]).
-      reflexivity.
-      do 2 (rewrite MapsPtes.F.add_neq_o;[ | intros abs;elim Heq4;rewrite abs;reflexivity]).
-      rewrite MapsPtes.F.add_neq_o;[ | intros abs;elim Heq3;rewrite abs;reflexivity].
-      reflexivity.
-      rewrite MapsPtes.F.add_neq_o;[ | intros abs;elim a_eq_b;rewrite abs;reflexivity].
-      rewrite Heq1.
-      intro k.
-      case(X.eq_dec k a);intros Heq3.
-      rewrite Heq3.
-      rewrite MapsPtes.F.add_eq_o;[ | reflexivity].
-      rewrite MapsPtes.F.add_neq_o;[ | intros abs;elim a_eq_b;rewrite abs;reflexivity].
-      rewrite MapsPtes.F.add_eq_o;[ | reflexivity].
-      reflexivity.
-      rewrite MapsPtes.F.add_neq_o;[ | intros abs;elim Heq3;rewrite abs;reflexivity].
-      case(X.eq_dec k b);intros Heq4.
-      rewrite Heq4.
-      repeat (rewrite MapsPtes.F.add_eq_o;[ | reflexivity]).
-      reflexivity.
-      do 2 (rewrite MapsPtes.F.add_neq_o;[ | intros abs;elim Heq4;rewrite abs;reflexivity]).
-      rewrite MapsPtes.F.add_neq_o;[ | intros abs;elim Heq3;rewrite abs;reflexivity].
-      reflexivity. }
+      * rewrite MapsPtes.F.add_neq_o;[ | intros abs;elim a_eq_b;rewrite abs;reflexivity].
+        rewrite Heq1.
+        intro k.
+        case(X.eq_dec k a);intros Heq3.
+        -- rewrite Heq3.
+           rewrite MapsPtes.F.add_eq_o;[ | reflexivity].
+           rewrite MapsPtes.F.add_neq_o;[ | intros abs;elim a_eq_b;rewrite abs;reflexivity].
+           rewrite MapsPtes.F.add_eq_o;[ | reflexivity].
+           reflexivity.
+        -- rewrite MapsPtes.F.add_neq_o;[ | intros abs;elim Heq3;rewrite abs;reflexivity].
+           case(X.eq_dec k b);intros Heq4.
+           ++ rewrite Heq4.
+              repeat (rewrite MapsPtes.F.add_eq_o;[ | reflexivity]).
+              reflexivity.
+           ++ do 2 (rewrite MapsPtes.F.add_neq_o;[ | intros abs;elim Heq4;rewrite abs;reflexivity]).
+              rewrite MapsPtes.F.add_neq_o;[ | intros abs;elim Heq3;rewrite abs;reflexivity].
+              reflexivity.
+      * rewrite MapsPtes.F.add_neq_o;[ | intros abs;elim a_eq_b;rewrite abs;reflexivity].
+        rewrite Heq1.
+        intro k.
+        case(X.eq_dec k a);intros Heq3.
+        -- rewrite Heq3.
+           rewrite MapsPtes.F.add_eq_o;[ | reflexivity].
+           rewrite MapsPtes.F.add_neq_o;[ | intros abs;elim a_eq_b;rewrite abs;reflexivity].
+           rewrite MapsPtes.F.add_eq_o;[ | reflexivity].
+           reflexivity.
+        -- rewrite MapsPtes.F.add_neq_o;[ | intros abs;elim Heq3;rewrite abs;reflexivity].
+           case(X.eq_dec k b);intros Heq4.
+           ++ rewrite Heq4.
+              repeat (rewrite MapsPtes.F.add_eq_o;[ | reflexivity]).
+              reflexivity.
+           ++ do 2 (rewrite MapsPtes.F.add_neq_o;[ | intros abs;elim Heq4;rewrite abs;reflexivity]).
+              rewrite MapsPtes.F.add_neq_o;[ | intros abs;elim Heq3;rewrite abs;reflexivity].
+              reflexivity.
   Qed.
 
   Lemma add_comm : forall a b ms, eq (add a (add b ms)) (add b (add a ms)).
@@ -519,52 +512,44 @@ Module PreMake(X:OrderedType)(Maps:FMapInterface.S with Module E:=X) <: S(X).
       Maps.Equal (Maps.fold f ms1 ms2) (Maps.fold f ms1' ms2').
   Proof.
     intros f f_morph f_proper f_transpose (* f_in *) f_in' ms1 ms1' H1 ms2 ms2' H2.
-
     revert ms1' H1 ms2' H2.
     pattern ms1,(Maps.fold f ms1 ms2).
     apply MapsPtes.fold_rec.
-
-    { intros m H ms1' H1 ms2' H2.
+    - intros m H ms1' H1 ms2' H2.
       rewrite MapsPtes.fold_Empty.
-      assumption.    
-      auto with *.
-      rewrite <- H1.
-      assumption. }
-
-    { intros k e a m' m'' H H0 H1 H2 ms1' H3 ms2' H4.
+      + assumption.
+      + auto with *.
+      + rewrite <- H1.
+        assumption.
+    - intros k e a m' m'' H H0 H1 H2 ms1' H3 ms2' H4.
       intros k'.
       case (X.eq_dec k k');intros k_eq_k'.
-      rewrite <- k_eq_k' in *.
-      assert (Equivalence (@Maps.Equal nat)).
-      auto with *.
-
-      rewrite (@MapsPtes.fold_Add nat _ (@Maps.Equal nat) H5 f f_proper f_transpose  m' ms1' k e);trivial .
-      apply (f_morph k k' e a (Maps.fold f m' ms2'));trivial.
-      apply H2;trivial.
-      reflexivity.
-      
-      intro k''. 
-      rewrite <- H3.
-      apply H1.    
-
-
-      rewrite f_in'.
-      assert(MapsPtes.Add k e m' ms1').
-      intro k''. 
-      rewrite <- H3.
-      apply H1.    
-      rewrite MapsPtes.fold_Add.    
-      6:eexact H5.
-      rewrite f_in'.
-      apply H2.
-      reflexivity.
-      assumption.
-      assumption.
-      auto with *.
-      assumption.
-      assumption.
-      assumption.
-      assumption. }
+      + rewrite <- k_eq_k' in *.
+        assert (Equivalence (@Maps.Equal nat)) by auto with *.
+        rewrite (@MapsPtes.fold_Add nat _ (@Maps.Equal nat) H5 f f_proper f_transpose  m' ms1' k e);trivial .
+        * apply (f_morph k k' e a (Maps.fold f m' ms2'));trivial.
+          apply H2;trivial.
+          reflexivity.
+        * intro k''.
+          rewrite <- H3.
+          apply H1.
+      + rewrite f_in'.
+        * assert(MapsPtes.Add k e m' ms1').
+          { intro k''.
+            rewrite <- H3.
+            apply H1. }
+          rewrite MapsPtes.fold_Add.
+          6:{ eexact H5. }
+          -- rewrite f_in'.
+             ++ apply H2.
+                ** reflexivity.
+                ** assumption.
+             ++ assumption.
+          -- auto with *.
+          -- assumption.
+          -- assumption.
+          -- assumption.
+        * assumption.
   Qed.
 
   Lemma empty_no_mem : forall a, mem a empty = false.
@@ -588,7 +573,7 @@ Module PreMake(X:OrderedType)(Maps:FMapInterface.S with Module E:=X) <: S(X).
       Maps.Equal (Maps.fold add_multiple ms1 ms2) (Maps.fold add_multiple ms1' ms2')).
     apply fold_pseudo_morph.
     intros k k' n ms0 ms'0 H H0.
-    apply add_multiple_morph;trivial.
+    now apply add_multiple_morph.
     apply add_multiple_morph_Proper.
     apply transpose_neqkey_equal_add_multiple.
     intros k e a k' H.
@@ -599,10 +584,10 @@ Module PreMake(X:OrderedType)(Maps:FMapInterface.S with Module E:=X) <: S(X).
 
     pattern ms,(Maps.fold add_multiple ms (Maps.empty nat)).
     apply MapsPtes.fold_rec_bis.
-    
+
     intros.
     transitivity m;assumption.
-    
+
     reflexivity.
 
 
@@ -638,7 +623,7 @@ Module PreMake(X:OrderedType)(Maps:FMapInterface.S with Module E:=X) <: S(X).
     case(X.eq_dec k a);intro Heq2.
     rewrite MapsPtes.F.add_eq_o;[|symmetry;assumption].
     rewrite MapsPtes.F.add_eq_o;[|symmetry;assumption].
-    f_equal;omega.
+    f_equal;lia.
     do 3 (rewrite MapsPtes.F.add_neq_o;[|intros abs;elim Heq2;rewrite abs;reflexivity]).
     reflexivity.
     rewrite MapsPtes.F.add_eq_o;[|reflexivity].
@@ -650,7 +635,7 @@ Module PreMake(X:OrderedType)(Maps:FMapInterface.S with Module E:=X) <: S(X).
     do 3 (rewrite MapsPtes.F.add_neq_o;[|intros abs;elim Heq2;rewrite abs;reflexivity]).
     reflexivity.
   Qed.
-    
+
   Lemma add_add_add: 
     forall k k' v v' (m:t), 
       X.eq k k' ->
@@ -680,7 +665,7 @@ Module PreMake(X:OrderedType)(Maps:FMapInterface.S with Module E:=X) <: S(X).
     clear.
     apply fold_pseudo_morph.
     intros k k' n ms0 ms'0 H H0.
-    apply add_multiple_morph;trivial.
+    now apply add_multiple_morph.
     apply add_multiple_morph_Proper.
     apply transpose_neqkey_equal_add_multiple.
     intros k e a k' H.
@@ -688,107 +673,106 @@ Module PreMake(X:OrderedType)(Maps:FMapInterface.S with Module E:=X) <: S(X).
     destruct (Maps.find k a).
     apply MapsPtes.F.add_neq_o;trivial.
     apply MapsPtes.F.add_neq_o;trivial.
-  
+
     pattern m1,(Maps.fold add_multiple m1 m2).
     apply MapsPtes.fold_rec.
 
-    { intros m H k e.
+    - intros m H k e.
       unfold add_multiple at 2.
       replace (Maps.find k m) with (@None nat) by (symmetry;apply Empty_not_find;assumption).
       rewrite MapsPtes.fold_Add with (m1:=m) (k:=k) (e:=e);auto with *.
-      rewrite MapsPtes.fold_Empty;auto with *.
-      apply transpose_neqkey_equal_add_multiple.
-      intros abs.
-      red in abs.
-      destruct abs as [v H1];elim (H k v H1).
-      red;tauto. }
-
-    { intros k e a m' m'' H H0 H1 H2 k0 e0.
-      rewrite morph with (ms1':= (add_multiple k0 e0 (add_multiple k e m')))
-        (ms2':=m2);trivial; try reflexivity.
-      case (X.eq_dec k k0);intro Heq.
-      unfold add_multiple at 2 3 4 5.
-      case_eq (Maps.find k a);[intro n|];intro Heq1.
-      rewrite <- Heq.
-      rewrite (MapsPtes.F.not_find_in_iff m' k) in H0.
-      rewrite H0.
-      do 2 (rewrite MapsPtes.F.add_eq_o;[|reflexivity]).
-      rewrite morph with (ms1':=(add_multiple k0 (S (e0 + e)) m')) (ms2':=m2);trivial;try reflexivity. 
-      rewrite (H2 k0 (S (e0+e))). 
-      rewrite Heq.
-      rewrite add_add_add.
-      unfold add_multiple.
-      rewrite Heq in Heq1;rewrite Heq1.
-      replace ((S(e0 + e) + n)) with (e0 + (S (e + n))) by omega.
-      reflexivity.
-      reflexivity.
-      rewrite add_add_add.
-      unfold add_multiple.
-      rewrite  Heq in H0.
-      rewrite H0.
-      reflexivity.
-      rewrite <- Heq;reflexivity.
-      rewrite <- Heq.
-      rewrite (MapsPtes.F.not_find_in_iff m' k) in H0.
-      rewrite H0.
-      do 2 (rewrite MapsPtes.F.add_eq_o;[|reflexivity]).
-      rewrite morph with (ms1':=(add_multiple k0 (S(e0 + e)) m')) (ms2':=m2);trivial;try reflexivity. 
-      rewrite (H2 k0 (S(e0+e))). 
-      rewrite Heq.
-      rewrite add_add_add.
-      unfold add_multiple.
-      rewrite Heq in Heq1;rewrite Heq1.
-      reflexivity.
-      reflexivity.
-      rewrite add_add_add.
-      unfold add_multiple.
-      rewrite  Heq in H0.
-      rewrite H0.
-      reflexivity.
-      rewrite <- Heq;reflexivity.
-      rewrite morph with (ms1':= (add_multiple k e (add_multiple k0 e0 m')))
-        (ms2':=m2);trivial;try reflexivity.    
-      rewrite MapsPtes.fold_Add with (k:=k) (e:=e) (m1:=(add_multiple k0 e0 m'));auto with *.
-      rewrite H2.
-      rewrite add_multiple_comm;reflexivity.
-      apply transpose_neqkey_equal_add_multiple.
-      unfold add_multiple.
-      destruct (Maps.find k0 m').
-      rewrite MapsPtes.F.add_in_iff.
-      intros abs;destruct abs.
-      apply Heq;rewrite H3;reflexivity.
-      apply H0;apply H3.
-      rewrite MapsPtes.F.add_in_iff.
-      intros abs;destruct abs.
-      apply Heq;rewrite H3;reflexivity.
-      apply H0;apply H3.
-      red.
-      intro y.
-      replace  (Maps.add k e (add_multiple k0 e0 m')) with 
-        (add_multiple k e (add_multiple k0 e0 m')).
-      rewrite add_multiple_comm;reflexivity.
-      unfold  add_multiple at 1.
-      assert (~Maps.In k (add_multiple k0 e0 m')).
-      unfold add_multiple.
-      destruct (Maps.find k0 m').
-      rewrite MapsPtes.F.add_in_iff.
-      intros abs;destruct abs.
-      apply Heq;rewrite H3;reflexivity.
-      apply H0;apply H3.
-      rewrite MapsPtes.F.add_in_iff.
-      intros abs;destruct abs.
-      apply Heq;rewrite H3;reflexivity.
-      apply H0;apply H3.
-      rewrite MapsPtes.F.not_find_in_iff in H3.
-      rewrite H3;reflexivity.
-      rewrite add_multiple_comm;reflexivity.
-      setoid_replace m'' with (add_multiple k e m').
-      reflexivity.
-      replace (add_multiple k e m') with (Maps.add k e m').
-      apply H1.
-      unfold add_multiple.
-      rewrite MapsPtes.F.not_find_in_iff in H0.
-      rewrite H0;reflexivity. }
+      + rewrite MapsPtes.fold_Empty;auto with *.
+      + apply transpose_neqkey_equal_add_multiple.
+      + intros abs.
+        red in abs.
+        destruct abs as [v H1];elim (H k v H1).
+      + red;tauto.
+    - intros k e a m' m'' H H0 H1 H2 k0 e0.
+    rewrite morph with (ms1':= (add_multiple k0 e0 (add_multiple k e m')))
+      (ms2':=m2);trivial; try reflexivity.
+    case (X.eq_dec k k0);intro Heq.
+    unfold add_multiple at 2 3 4 5.
+    case_eq (Maps.find k a);[intro n|];intro Heq1.
+    rewrite <- Heq.
+    rewrite (MapsPtes.F.not_find_in_iff m' k) in H0.
+    rewrite H0.
+    do 2 (rewrite MapsPtes.F.add_eq_o;[|reflexivity]).
+    rewrite morph with (ms1':=(add_multiple k0 (S (e0 + e)) m')) (ms2':=m2);trivial;try reflexivity. 
+    rewrite (H2 k0 (S (e0+e))). 
+    rewrite Heq.
+    rewrite add_add_add.
+    unfold add_multiple.
+    rewrite Heq in Heq1;rewrite Heq1.
+    replace ((S(e0 + e) + n)) with (e0 + (S (e + n))) by lia.
+    reflexivity.
+    reflexivity.
+    rewrite add_add_add.
+    unfold add_multiple.
+    rewrite  Heq in H0.
+    rewrite H0.
+    reflexivity.
+    rewrite <- Heq;reflexivity.
+    rewrite <- Heq.
+    rewrite (MapsPtes.F.not_find_in_iff m' k) in H0.
+    rewrite H0.
+    do 2 (rewrite MapsPtes.F.add_eq_o;[|reflexivity]).
+    rewrite morph with (ms1':=(add_multiple k0 (S(e0 + e)) m')) (ms2':=m2);trivial;try reflexivity. 
+    rewrite (H2 k0 (S(e0+e))). 
+    rewrite Heq.
+    rewrite add_add_add.
+    unfold add_multiple.
+    rewrite Heq in Heq1;rewrite Heq1.
+    reflexivity.
+    reflexivity.
+    rewrite add_add_add.
+    unfold add_multiple.
+    rewrite  Heq in H0.
+    rewrite H0.
+    reflexivity.
+    rewrite <- Heq;reflexivity.
+    rewrite morph with (ms1':= (add_multiple k e (add_multiple k0 e0 m')))
+      (ms2':=m2);trivial;try reflexivity.    
+    rewrite MapsPtes.fold_Add with (k:=k) (e:=e) (m1:=(add_multiple k0 e0 m'));auto with *.
+    rewrite H2.
+    rewrite add_multiple_comm;reflexivity.
+    apply transpose_neqkey_equal_add_multiple.
+    unfold add_multiple.
+    destruct (Maps.find k0 m').
+    rewrite MapsPtes.F.add_in_iff.
+    intros abs;destruct abs.
+    apply Heq;rewrite H3;reflexivity.
+    apply H0;apply H3.
+    rewrite MapsPtes.F.add_in_iff.
+    intros abs;destruct abs.
+    apply Heq;rewrite H3;reflexivity.
+    apply H0;apply H3.
+    red.
+    intro y.
+    replace  (Maps.add k e (add_multiple k0 e0 m')) with 
+       (add_multiple k e (add_multiple k0 e0 m')).
+    rewrite add_multiple_comm;reflexivity.
+    unfold  add_multiple at 1.
+    assert (~Maps.In k (add_multiple k0 e0 m')).
+    unfold add_multiple.
+    destruct (Maps.find k0 m').
+    rewrite MapsPtes.F.add_in_iff.
+    intros abs;destruct abs.
+    apply Heq;rewrite H3;reflexivity.
+    apply H0;apply H3.
+    rewrite MapsPtes.F.add_in_iff.
+    intros abs;destruct abs.
+    apply Heq;rewrite H3;reflexivity.
+    apply H0;apply H3.
+    rewrite MapsPtes.F.not_find_in_iff in H3.
+    rewrite H3;reflexivity.
+    rewrite add_multiple_comm;reflexivity.
+    setoid_replace m'' with (add_multiple k e m').
+    reflexivity.
+    replace (add_multiple k e m') with (Maps.add k e m').
+    apply H1.
+    unfold add_multiple.
+    rewrite MapsPtes.F.not_find_in_iff in H0.
+    rewrite H0;reflexivity.
   Qed.
 
   Lemma union_rec_left : forall a ms ms', eq (union (add a ms) ms') (add a (union ms ms')).
@@ -815,7 +799,7 @@ Module PreMake(X:OrderedType)(Maps:FMapInterface.S with Module E:=X) <: S(X).
     clear.
     apply fold_pseudo_morph.
     intros k k' n ms0 ms'0 H H0.
-    apply add_multiple_morph;trivial.
+    now apply add_multiple_morph.
     apply add_multiple_morph_Proper.
     apply transpose_neqkey_equal_add_multiple.
     intros k e a k' H.
@@ -823,14 +807,12 @@ Module PreMake(X:OrderedType)(Maps:FMapInterface.S with Module E:=X) <: S(X).
     destruct (Maps.find k a).
     apply MapsPtes.F.add_neq_o;trivial.
     apply MapsPtes.F.add_neq_o;trivial.
-  
+
     pattern m1,(Maps.fold add_multiple m1 m2).
     apply MapsPtes.fold_rec.
-
-    { intros m H k e.
-      rewrite MapsPtes.fold_Empty;auto with *. }
-
-    { intros k e a m' m'' H H0 H1 H2 k0 e0.
+    - intros m H k e.
+      rewrite MapsPtes.fold_Empty;auto with *.
+    - intros k e a m' m'' H H0 H1 H2 k0 e0.
       rewrite morph with (ms1':= (add_multiple k e m'))
         (ms2':=(add_multiple k0 e0 m2));trivial; try reflexivity.
       rewrite MapsPtes.fold_Add with (k:=k) (e:=e) (m1:= m');auto with *.
@@ -844,7 +826,7 @@ Module PreMake(X:OrderedType)(Maps:FMapInterface.S with Module E:=X) <: S(X).
       unfold add_multiple.
       rewrite (MapsPtes.F.not_find_in_iff m' k) in H0.
       rewrite H0.
-      exact H1. }
+      exact H1.
   Qed.
 
   Lemma union_rec_right : forall a ms ms', eq (union ms (add a ms')) (add a (union ms ms')).
@@ -921,7 +903,7 @@ Qed.
     case_eq (Maps.find φ' Γ).
 
     intros n Heq.
-    rewrite MapsFact.add_eq_o.    
+    rewrite MapsFact.add_eq_o.
     simpl.
     rewrite MapsFact.Equal_mapsto_iff.
     intros k e.
@@ -956,7 +938,7 @@ Qed.
     auto.
 
     intros Heq.
-    rewrite MapsFact.add_eq_o.    
+    rewrite MapsFact.add_eq_o.
     rewrite MapsFact.Equal_mapsto_iff.
     intros k e.
     case (X.eq_dec k φ);intros Heq'.
@@ -965,11 +947,11 @@ Qed.
     rewrite MapsFact.remove_eq_o in H0.
     discriminate.
     symmetry;assumption.
-    rewrite MapsPtes.F.find_mapsto_iff in H0.    
+    rewrite MapsPtes.F.find_mapsto_iff in H0.
     rewrite (MapsPtes.F.find_o _ Heq') in H0.
     rewrite (MapsPtes.F.find_o _ H) in H0.
     rewrite Heq in H0;discriminate.
-    do 2 rewrite MapsPtes.F.find_mapsto_iff.    
+    do 2 rewrite MapsPtes.F.find_mapsto_iff.
     rewrite MapsPtes.F.remove_neq_o.
     rewrite MapsPtes.F.add_neq_o.
     tauto.
@@ -980,7 +962,7 @@ Qed.
     symmetry;assumption.
   Qed.
 
-  Lemma remove_diff_add : forall φ φ' Γ, ~X.eq φ φ' -> 
+  Lemma remove_diff_add : forall φ φ' Γ, ~X.eq φ φ' ->
     eq (remove φ (add φ' Γ)) (add φ' (remove φ Γ)).
   Proof.
     intros φ φ' Γ H.
@@ -991,127 +973,118 @@ Qed.
       [intros n|]; intros Heq;
         (case_eq (Maps.find φ Γ);
           [intros n'|];intros Heq').
-    destruct n'.
-
-    { rewrite MapsFact.add_neq_o;[|intro;elim H;symmetry;assumption].    
-      rewrite Heq'.
-      rewrite MapsFact.remove_neq_o;[| assumption].
-      rewrite Heq.
-      rewrite MapsFact.Equal_mapsto_iff.
-      intros k e.
-      do 2 rewrite MapsFact.find_mapsto_iff.
-      case (X.eq_dec k φ); case (X.eq_dec k φ');intros Heq1 Heq2.
-      elim H;apply X.eq_trans with k.
-      symmetry;assumption.
-      assumption.
-      rewrite MapsFact.remove_eq_o;[|symmetry;assumption ].
-      rewrite MapsFact.add_neq_o;[|intro;elim Heq1;symmetry;assumption ].
-      rewrite MapsFact.remove_eq_o;[|symmetry;assumption ].
-      reflexivity.
-      rewrite MapsFact.remove_neq_o;[|intro;elim Heq2;symmetry;assumption ].
-      rewrite MapsFact.add_eq_o;[|symmetry;assumption ].
-      rewrite MapsFact.add_eq_o;[|symmetry;assumption ].
-      reflexivity.
-      rewrite MapsFact.remove_neq_o;[|intro;elim Heq2;symmetry;assumption ].
-      rewrite MapsFact.add_neq_o;[|intro;elim Heq1;symmetry;assumption ].
-      rewrite MapsFact.add_neq_o;[|intro;elim Heq1;symmetry;assumption ].
-      rewrite MapsFact.remove_neq_o;[|intro;elim Heq2;symmetry;assumption ].
-      reflexivity. }
-
-    { rewrite MapsFact.add_neq_o;[|intro;elim H;symmetry;assumption].    
-      rewrite Heq'.
-      rewrite MapsFact.add_neq_o;[| assumption].
-      rewrite Heq.
-      rewrite MapsFact.Equal_mapsto_iff.
-      intros k e.
-      do 2 rewrite MapsFact.find_mapsto_iff.
-      case (X.eq_dec k φ); case (X.eq_dec k φ');intros Heq1 Heq2.
-      elim H;apply X.eq_trans with k.
-      symmetry;assumption.
-      assumption.
-      rewrite MapsFact.add_eq_o;[|symmetry;assumption ].
-      rewrite MapsFact.add_neq_o;[|intro;elim Heq1;symmetry;assumption ].
-      rewrite MapsFact.add_eq_o;[|symmetry;assumption ].
-      reflexivity.
-      rewrite MapsFact.add_neq_o;[|intro;elim Heq2;symmetry;assumption ].
-      rewrite MapsFact.add_eq_o;[|symmetry;assumption ].
-      rewrite MapsFact.add_eq_o;[|symmetry;assumption ].
-      reflexivity.
-      rewrite MapsFact.add_neq_o;[|intro;elim Heq2;symmetry;assumption ].
-      rewrite MapsFact.add_neq_o;[|intro;elim Heq1;symmetry;assumption ].
-      rewrite MapsFact.add_neq_o;[|intro;elim Heq1;symmetry;assumption ].
-      rewrite MapsFact.add_neq_o;[|intro;elim Heq2;symmetry;assumption ].
-      reflexivity. }
-
-    { rewrite MapsFact.add_neq_o;[|intro;elim H;symmetry;assumption].    
+    - destruct n'.
+      + rewrite MapsFact.add_neq_o;[|intro;elim H;symmetry;assumption].
+        rewrite Heq'.
+        rewrite MapsFact.remove_neq_o;[| assumption].
+        rewrite Heq.
+        rewrite MapsFact.Equal_mapsto_iff.
+        intros k e.
+        do 2 rewrite MapsFact.find_mapsto_iff.
+        case (X.eq_dec k φ); case (X.eq_dec k φ');intros Heq1 Heq2.
+        * elim H;apply X.eq_trans with k.
+          -- symmetry;assumption.
+          -- assumption.
+        * rewrite MapsFact.remove_eq_o;[|symmetry;assumption ].
+          rewrite MapsFact.add_neq_o;[|intro;elim Heq1;symmetry;assumption ].
+          rewrite MapsFact.remove_eq_o;[|symmetry;assumption ].
+          reflexivity.
+        * rewrite MapsFact.remove_neq_o;[|intro;elim Heq2;symmetry;assumption ].
+          rewrite MapsFact.add_eq_o;[|symmetry;assumption ].
+          rewrite MapsFact.add_eq_o;[|symmetry;assumption ].
+          reflexivity.
+        * rewrite MapsFact.remove_neq_o;[|intro;elim Heq2;symmetry;assumption ].
+          rewrite MapsFact.add_neq_o;[|intro;elim Heq1;symmetry;assumption ].
+          rewrite MapsFact.add_neq_o;[|intro;elim Heq1;symmetry;assumption ].
+          rewrite MapsFact.remove_neq_o;[|intro;elim Heq2;symmetry;assumption ].
+          reflexivity.
+      + rewrite MapsFact.add_neq_o;[|intro;elim H;symmetry;assumption].
+        rewrite Heq'.
+        rewrite MapsFact.add_neq_o;[| assumption].
+        rewrite Heq.
+        rewrite MapsFact.Equal_mapsto_iff.
+        intros k e.
+        do 2 rewrite MapsFact.find_mapsto_iff.
+        case (X.eq_dec k φ); case (X.eq_dec k φ');intros Heq1 Heq2.
+        * elim H;apply X.eq_trans with k.
+          -- symmetry;assumption.
+          -- assumption.
+        * rewrite MapsFact.add_eq_o;[|symmetry;assumption ].
+          rewrite MapsFact.add_neq_o;[|intro;elim Heq1;symmetry;assumption ].
+          rewrite MapsFact.add_eq_o;[|symmetry;assumption ].
+          reflexivity.
+        * rewrite MapsFact.add_neq_o;[|intro;elim Heq2;symmetry;assumption ].
+          rewrite MapsFact.add_eq_o;[|symmetry;assumption ].
+          rewrite MapsFact.add_eq_o;[|symmetry;assumption ].
+          reflexivity.
+        * rewrite MapsFact.add_neq_o;[|intro;elim Heq2;symmetry;assumption ].
+          rewrite MapsFact.add_neq_o;[|intro;elim Heq1;symmetry;assumption ].
+          rewrite MapsFact.add_neq_o;[|intro;elim Heq1;symmetry;assumption ].
+          rewrite MapsFact.add_neq_o;[|intro;elim Heq2;symmetry;assumption ].
+          reflexivity.
+    - rewrite MapsFact.add_neq_o;[|intro;elim H;symmetry;assumption].
       rewrite Heq.
       rewrite Heq'.
-      apply MapsPtes.F.Equal_refl. }
-
-
-
-    rewrite MapsFact.add_neq_o;[|intro;elim H;symmetry;assumption].    
-    rewrite Heq'.
-    destruct n'.
-
-    { rewrite MapsFact.remove_neq_o;[|intro;elim H;assumption].    
-      rewrite Heq.
-      rewrite MapsFact.Equal_mapsto_iff.
-      intros k e.
-      do 2 rewrite MapsFact.find_mapsto_iff.
-      case (X.eq_dec k φ); case (X.eq_dec k φ');intros Heq1 Heq2.
-      elim H;apply X.eq_trans with k.
-      symmetry;assumption.
-      assumption.
-      rewrite MapsFact.add_neq_o;[|intro;elim Heq1;symmetry;assumption ].
-      rewrite MapsFact.remove_eq_o;[|symmetry;assumption ].
-      rewrite MapsFact.remove_eq_o;[|symmetry;assumption ].
-      reflexivity.
-      rewrite MapsFact.remove_neq_o;[|intro;elim Heq2;symmetry;assumption ].
-      rewrite MapsFact.add_eq_o;[|symmetry;assumption ].
-      rewrite MapsFact.add_eq_o;[|symmetry;assumption ].
-      reflexivity.
-      rewrite MapsFact.remove_neq_o;[|intro;elim Heq2;symmetry;assumption ].
-      rewrite MapsFact.add_neq_o;[|intro;elim Heq1;symmetry;assumption ].
-      rewrite MapsFact.add_neq_o;[|intro;elim Heq1;symmetry;assumption ].
-      rewrite MapsFact.remove_neq_o;[|intro;elim Heq2;symmetry;assumption ].
-      reflexivity. }
-
-    { rewrite MapsFact.add_neq_o;[|intro;elim H;assumption].    
-      rewrite Heq.
-      rewrite MapsFact.Equal_mapsto_iff.
-      intros k e.
-      do 2 rewrite MapsFact.find_mapsto_iff.
-      case (X.eq_dec k φ); case (X.eq_dec k φ');intros Heq1 Heq2.
-      elim H;apply X.eq_trans with k.
-      symmetry;assumption.
-      assumption.
-      rewrite MapsFact.add_eq_o;[|symmetry;assumption ].
-      rewrite MapsFact.add_neq_o;[|intro;elim Heq1;symmetry;assumption ].
-      rewrite MapsFact.add_eq_o;[|symmetry;assumption ].
-      reflexivity.
-      rewrite MapsFact.add_neq_o;[|intro;elim Heq2;symmetry;assumption ].
-      rewrite MapsFact.add_eq_o;[|symmetry;assumption ].
-      rewrite MapsFact.add_eq_o;[|symmetry;assumption ].
-      reflexivity.
-      rewrite MapsFact.add_neq_o;[|intro;elim Heq2;symmetry;assumption ].
-      rewrite MapsFact.add_neq_o;[|intro;elim Heq1;symmetry;assumption ].
-      rewrite MapsFact.add_neq_o;[|intro;elim Heq1;symmetry;assumption ].
-      rewrite MapsFact.add_neq_o;[|intro;elim Heq2;symmetry;assumption ].
-      reflexivity. }
-
-    { rewrite MapsFact.add_neq_o;[|intro;elim H;symmetry;assumption  ].    
+      apply MapsPtes.F.Equal_refl.
+    - rewrite MapsFact.add_neq_o;[|intro;elim H;symmetry;assumption].    
+      rewrite Heq'.
+      destruct n'.
+      + rewrite MapsFact.remove_neq_o;[|intro;elim H;assumption].    
+        rewrite Heq.
+        rewrite MapsFact.Equal_mapsto_iff.
+        intros k e.
+        do 2 rewrite MapsFact.find_mapsto_iff.
+        case (X.eq_dec k φ); case (X.eq_dec k φ');intros Heq1 Heq2.
+        * elim H;apply X.eq_trans with k.
+          -- symmetry;assumption.
+          -- assumption.
+        * rewrite MapsFact.add_neq_o;[|intro;elim Heq1;symmetry;assumption ].
+          rewrite MapsFact.remove_eq_o;[|symmetry;assumption ].
+          rewrite MapsFact.remove_eq_o;[|symmetry;assumption ].
+          reflexivity.
+        * rewrite MapsFact.remove_neq_o;[|intro;elim Heq2;symmetry;assumption ].
+          rewrite MapsFact.add_eq_o;[|symmetry;assumption ].
+          rewrite MapsFact.add_eq_o;[|symmetry;assumption ].
+          reflexivity.
+        * rewrite MapsFact.remove_neq_o;[|intro;elim Heq2;symmetry;assumption ].
+          rewrite MapsFact.add_neq_o;[|intro;elim Heq1;symmetry;assumption ].
+          rewrite MapsFact.add_neq_o;[|intro;elim Heq1;symmetry;assumption ].
+          rewrite MapsFact.remove_neq_o;[|intro;elim Heq2;symmetry;assumption ].
+          reflexivity.
+      + rewrite MapsFact.add_neq_o;[|intro;elim H;assumption].    
+        rewrite Heq.
+        rewrite MapsFact.Equal_mapsto_iff.
+        intros k e.
+        do 2 rewrite MapsFact.find_mapsto_iff.
+        case (X.eq_dec k φ); case (X.eq_dec k φ');intros Heq1 Heq2.
+        * elim H;apply X.eq_trans with k.
+          -- symmetry;assumption.
+          -- assumption.
+        * rewrite MapsFact.add_eq_o;[|symmetry;assumption ].
+          rewrite MapsFact.add_neq_o;[|intro;elim Heq1;symmetry;assumption ].
+          rewrite MapsFact.add_eq_o;[|symmetry;assumption ].
+          reflexivity.
+        * rewrite MapsFact.add_neq_o;[|intro;elim Heq2;symmetry;assumption ].
+          rewrite MapsFact.add_eq_o;[|symmetry;assumption ].
+          rewrite MapsFact.add_eq_o;[|symmetry;assumption ].
+          reflexivity.
+        * rewrite MapsFact.add_neq_o;[|intro;elim Heq2;symmetry;assumption ].
+          rewrite MapsFact.add_neq_o;[|intro;elim Heq1;symmetry;assumption ].
+          rewrite MapsFact.add_neq_o;[|intro;elim Heq1;symmetry;assumption ].
+          rewrite MapsFact.add_neq_o;[|intro;elim Heq2;symmetry;assumption ].
+          reflexivity.
+    - rewrite MapsFact.add_neq_o;[|intro;elim H;symmetry;assumption  ].
       rewrite Heq.
       rewrite Heq'.
-      reflexivity. }
+      reflexivity.
   Qed.
-  
+
   Lemma is_empty_morph_eq : forall (Γ Γ' : t), eq Γ Γ' -> is_empty Γ = is_empty Γ'.
   Proof.
     unfold eq,is_empty.
     apply MapsFact.is_empty_m.
   Qed.
-    
+
   Lemma remove_morph_eq : 
     forall a a', X.eq a a' -> forall ms ms',  eq ms ms' -> eq (remove a ms) (remove a' ms'). 
   Proof.
@@ -1130,21 +1103,18 @@ Qed.
     intros a ms ms'.
     unfold mem,union.
     apply MapsPtes.fold_rec.
-
-    { intros m H H0.
+    - intros m H H0.
       apply Maps.mem_2 in H0.
       rewrite MapsPtes.F.in_find_iff in H0.
       rewrite Empty_not_find in H0.
       elim H0;reflexivity.
-      assumption. }
-
-    {
-      intros k e a0 m' m'' H H0 H1 H2 H3.
+      assumption.
+    - intros k e a0 m' m'' H H0 H1 H2 H3.
       unfold mem,add,add_multiple.
-      destruct (Maps.find k a0).    
+      destruct (Maps.find k a0).
       case (X.eq_dec a k);intros heq.
-      rewrite MapsPtes.F.add_eq_b;auto.
-      rewrite MapsPtes.F.add_neq_b;auto.
+      now rewrite MapsPtes.F.add_eq_b.
+      rewrite MapsPtes.F.add_neq_b by intuition.
       apply H2.
       red in H1.
       generalize (H1 a).
@@ -1155,21 +1125,20 @@ Qed.
       intros.
       rewrite <- H4.
       reflexivity.
-      auto.
+      intuition.
       case (X.eq_dec a k);intros heq.
-      rewrite MapsPtes.F.add_eq_b;auto.
-      rewrite MapsPtes.F.add_neq_b;auto.
+      now rewrite MapsPtes.F.add_eq_b.
+      rewrite MapsPtes.F.add_neq_b by intuition.
       apply H2.
       red in H1.
       generalize (H1 a).
       rewrite (MapsFact.mem_find_b) in H3. 
       destruct (Maps.find a m'');try discriminate.
-      rewrite MapsPtes.F.add_neq_o.
+      rewrite MapsPtes.F.add_neq_o by intuition.
       rewrite MapsFact.mem_find_b.
       intros.
       rewrite <- H4.
       reflexivity.
-      auto. }
   Qed.
 
   Lemma mem_union_r : forall a ms ms', mem a ms' = true -> mem a (union ms ms') = true.
@@ -1177,18 +1146,16 @@ Qed.
     intros a ms ms'.
     unfold mem,union.
     apply MapsPtes.fold_rec.
-
-    { tauto. }
-
-    { intros k e a0 m' m'' H H0 H1 H2 H3.
+    - tauto.
+    - intros k e a0 m' m'' H H0 H1 H2 H3.
       unfold mem,add,add_multiple.
-      destruct (Maps.find k a0).    
-      case (X.eq_dec a k);intros heq.
-      rewrite MapsPtes.F.add_eq_b;auto.
-      rewrite MapsPtes.F.add_neq_b;auto.
-      case ( X.eq_dec a k);intros.
-      apply  MapsPtes.F.add_eq_b;auto.
-      rewrite MapsPtes.F.add_neq_b;auto. }
+      destruct (Maps.find k a0).
+      + case (X.eq_dec a k);intros heq.
+        * now rewrite MapsPtes.F.add_eq_b.
+        * rewrite MapsPtes.F.add_neq_b by intuition; auto.
+      + case ( X.eq_dec a k);intros.
+        * now apply MapsPtes.F.add_eq_b.
+        * rewrite MapsPtes.F.add_neq_b by intuition; auto.
   Qed.
 
   Lemma mem_union_destruct : forall a ms ms', mem a (union ms ms') = true -> mem a ms = true \/mem a ms' = true.
@@ -1196,44 +1163,37 @@ Qed.
     intros a ms ms'.
     unfold mem,union,add_multiple.
     apply MapsPtes.fold_rec.
-
-    {
-      tauto.
-    }
-
-    {
-      intros k e a0 m' m''. 
+    - tauto.
+    - intros k e a0 m' m''.
       case (Maps.find k a0).
-      intros n H H0 H1 H2 H3.
-      case (X.eq_dec a k);intros heq.
-      red in H1.
-      rewrite MapsPtes.F.mem_find_b.
-      rewrite H1.
-      rewrite MapsPtes.F.add_eq_o;auto.
-      rewrite MapsPtes.F.add_neq_b in H3;auto.
-      destruct (H2 H3);auto.
-      left.
-      red in H1.
-      rewrite MapsPtes.F.mem_find_b.
-      rewrite H1.
-      rewrite MapsPtes.F.add_neq_o;auto.
-      rewrite <- MapsPtes.F.mem_find_b;auto.
-      intros H H0 H1 H2 H3.
-      case (X.eq_dec a k);intros heq.
-      red in H1.
-      rewrite MapsPtes.F.mem_find_b.
-      rewrite H1.
-      rewrite MapsPtes.F.add_eq_o;auto.
-      rewrite MapsPtes.F.add_neq_b in H3;auto.
-      destruct (H2 H3);auto.
-      left.
-      red in H1.
-      rewrite MapsPtes.F.mem_find_b.
-      rewrite H1.
-      rewrite MapsPtes.F.add_neq_o;auto.
-      rewrite <- MapsPtes.F.mem_find_b;auto.
-
-    }
+      + intros n H H0 H1 H2 H3.
+        case (X.eq_dec a k);intros heq.
+        * red in H1.
+          rewrite MapsPtes.F.mem_find_b.
+          rewrite H1.
+          now rewrite MapsPtes.F.add_eq_o; auto.
+        * rewrite MapsPtes.F.add_neq_b in H3 by intuition.
+          destruct (H2 H3);auto.
+          left.
+          red in H1.
+          rewrite MapsPtes.F.mem_find_b.
+          rewrite H1.
+          rewrite MapsPtes.F.add_neq_o by intuition.
+          now rewrite <- MapsPtes.F.mem_find_b.
+      + intros H H0 H1 H2 H3.
+        case (X.eq_dec a k);intros heq.
+        * red in H1.
+          rewrite MapsPtes.F.mem_find_b.
+          rewrite H1.
+          now rewrite MapsPtes.F.add_eq_o; auto.
+        * rewrite MapsPtes.F.add_neq_b in H3 by intuition.
+          destruct (H2 H3);auto.
+          left.
+          red in H1.
+          rewrite MapsPtes.F.mem_find_b.
+          rewrite H1.
+          rewrite MapsPtes.F.add_neq_o by intuition.
+          now rewrite <- MapsPtes.F.mem_find_b.
   Qed.
 
 
@@ -1244,27 +1204,27 @@ Qed.
     intros H.
     case (Maps.find b ms).
     intros [ | n].
-    rewrite MapsPtes.F.remove_neq_b;auto.
-    rewrite MapsPtes.F.add_neq_b;auto.
+    now rewrite MapsPtes.F.remove_neq_b by intuition.
+    now rewrite MapsPtes.F.add_neq_b by intuition.
     auto.
   Qed.
 
-  Lemma mem_remove_2 : forall a b ms, mem a (remove b ms) = true  -> mem a ms=true.
+  Lemma mem_remove_2 : forall a b ms, mem a (remove b ms) = true -> mem a ms=true.
   Proof.
     intros a b ms.
     unfold mem,remove.
     case_eq (Maps.find b ms);[intros n H|intros H].
     destruct n as [ | n].
     case (X.eq_dec a b);intros heq.
-    rewrite MapsPtes.F.remove_eq_b;auto;discriminate.
-    rewrite MapsPtes.F.remove_neq_b;auto.
+    now rewrite MapsPtes.F.remove_eq_b.
+    now rewrite MapsPtes.F.remove_neq_b by intuition.
     case (X.eq_dec a b);intros heq.
     intros _.
     rewrite MapsPtes.F.mem_find_b.
     rewrite <- (@MapsPtes.F.find_o _ _ _  _ heq) in H.
     rewrite H;reflexivity.
-    rewrite MapsPtes.F.add_neq_b;auto.
-    tauto.
+    now rewrite MapsPtes.F.add_neq_b by intuition.
+    trivial.
   Qed.
 
   Lemma eq_mem : forall ms ms', eq ms ms' -> (forall a, mem a ms = mem a ms').
@@ -1279,6 +1239,7 @@ Qed.
   Reserved Notation "∪" (at level 60, right associativity).
   Reserved Notation "∅" (at level 10, no associativity).
 
+  Declare Scope ILL_scope.
   Infix "∪" := union (at level 65, right associativity) : ILL_scope.
   Notation " a :: b " := (add a b) (at level 60, right associativity) : ILL_scope.
   Notation "{ a , .. , b }" := (add a .. (add b empty) ..) (at level 40): ILL_scope.
@@ -1291,18 +1252,18 @@ Qed.
 
   Notation " b '\' a " := (remove a b) (at level 64, right associativity) : ILL_scope.
   Open Scope ILL_scope.
-    
+
   Lemma multiset_ind : forall (P:t -> Type), (forall Γ Γ', Γ==Γ' -> P Γ -> P Γ') -> P empty -> (forall x Γ, P Γ -> P (x::Γ)) -> forall Γ, P Γ.
   Proof.
     intros P X X0 X1 Γ.
     induction Γ using MapsPtes.map_induction_bis.
-  
+
     eauto.
 
     apply X0.
 
     induction e as [| n].
-  
+
     generalize (X1 x Γ IHΓ).
     unfold add.
     rewrite MapsPtes.F.not_find_in_iff in H;rewrite H.
@@ -1324,15 +1285,15 @@ Qed.
   Proof.
     intros Γ.
     induction Γ using multiset_ind.
-    
+
     destruct IHΓ1.
     left;rewrite H in H0;assumption.
     right;destruct H0 as [φ [Γ' H1]];exists φ;exists Γ'.
     rewrite H in H1;assumption.
-    
-    
+
+
     left;reflexivity.
- 
+
     right.
     exists x.
     exists Γ.
@@ -1351,7 +1312,7 @@ Qed.
   Proof.
     exact add_morph_eq.
   Qed.
-  
+
   (* On peut réécrire à l'intérieur d'une union d'environnements. *)
   Add Morphism union
     with signature (eq==> eq ==> eq)
@@ -1442,7 +1403,7 @@ Qed.
  Qed.
 
 
-   
+
  Lemma union_singleton_decompose : 
    ∀ Δ Δ' φ, Δ∪Δ' == {φ} -> (Δ=={φ}/\Δ'==∅)\/(Δ'=={φ}/\Δ==∅).
  Proof.
@@ -1478,8 +1439,8 @@ Qed.
  Lemma mem_decompose : 
    forall Γ φ, φ ∈ Γ -> exists Γ', Γ == φ :: Γ'.
  Proof.
-   intros Γ. 
-   induction Γ using multiset_ind. 
+   intros Γ.
+   induction Γ using multiset_ind.
 
    intros φ H0.
    rewrite <- H in H0.
@@ -1502,7 +1463,7 @@ Qed.
    ∀ φ Γ Γ', φ::Γ == φ::Γ' -> Γ == Γ'.
  Proof.
    intros φ Γ Γ' H.
-   red in H.   
+   red in H.
    intro ψ.
    case (X.eq_dec ψ φ);intro Heq.
    rewrite Heq.
@@ -1530,7 +1491,7 @@ Qed.
    intros Γ'.
    rewrite <- H;auto.
    intros Γ'.
-   rewrite union_empty_right;rewrite union_empty_left;reflexivity.   
+   rewrite union_empty_right;rewrite union_empty_left;reflexivity.
 
    intros Γ'.
    rewrite union_rec_right;rewrite union_rec_left; rewrite IHΓ;reflexivity.
@@ -1542,7 +1503,7 @@ Qed.
    (exists Δ0, Δ' == φ :: Δ0 /\ Δ0∪Δ == Γ).
  Proof.
    intros Γ.
-   
+
    induction Γ using multiset_ind.
    intros Δ Δ' φ H0.   
    rewrite <- H in H0.
@@ -1567,15 +1528,15 @@ Qed.
    right;exists Δ0;split;auto.
    rewrite H2 in H.
    rewrite union_rec_right in H.
-   assert (H':=eq_add_inject _ _ _ H);clear H. 
+   assert (H':=eq_add_inject _ _ _ H);clear H.
    rewrite union_sym;assumption.
  Qed.
- 
+
  Lemma union_empty_decompose : ∀ Δ Δ', Δ∪Δ'== ∅ -> Δ==∅/\Δ'==∅.
  Proof.
    intros Δ.
    induction Δ using multiset_ind.
- 
+
    intros; rewrite <- H; rewrite <- H in H0;auto.
 
    intros Δ' H.
@@ -1693,23 +1654,23 @@ Lemma iter_transpose_neqkey :
 Proof.
   intros B eqB eqBeq f H H0.
   red.
-  intros k k' e e' a H1.  
+  intros k k' e e' a H1.
   induction e as [|e]; simpl.
   induction e' as [|e'];  simpl.
   apply H0;assumption.
   rewrite <- IHe'.
   apply H0;assumption.
-  
+
   rewrite IHe.
   clear IHe.
   induction e' as [|e'];  simpl in *.
   apply H0;assumption.
   rewrite <- IHe'.
   apply H0;assumption.
-Qed.  
+Qed.
 
 
-Lemma fold_morph : 
+Lemma fold_morph :
   ∀ (B : Type) (eqB : B → B → Prop),
   Equivalence eqB
   → (∀ f : A  → B → B,
@@ -1722,7 +1683,7 @@ Proof.
   revert m2 H2.
   unfold fold.
   apply MapsPtes.fold_rec_weak.
-  
+
   intros m m' a H2 H3 m2 H4.
   apply H3.
   rewrite H2;assumption.
@@ -1752,7 +1713,7 @@ Proof.
   apply iter_proper;assumption.
   apply iter_transpose_neqkey;assumption.
 
-Qed.    
+Qed.
 End PreMake.
 
 Module MakeAVL(X:OrderedType )<:S(X).
@@ -1832,8 +1793,8 @@ Module MakeRawList(X:OrderedType)<:S(X).
           | _ => mem e ms'
         end
     end.
-  
-  Inductive eq' : t -> t -> Prop := 
+
+  Inductive eq' : t -> t -> Prop :=
   | Eq_nil : eq' nil nil 
   | Eq_cons : forall e1 e2 ms1 ms2 ms2', X.eq e1 e2 -> eq' ms1 (ms2++ms2') -> eq' (e1::ms1) (ms2++e2::ms2').
 
@@ -1862,7 +1823,7 @@ Module MakeRawList(X:OrderedType)<:S(X).
     simpl. reflexivity.
   Qed.
 
-  Lemma find_decomp_concat : forall e e' ms m m' acc, find_decomp e ms acc = Some(e',m,m') -> 
+  Lemma find_decomp_concat : forall e e' ms m m' acc, find_decomp e ms acc = Some(e',m,m') ->
     (List.rev acc)++ms = m++e'::m'.
   Proof.
     intros e e' ms m m' acc.
@@ -1879,8 +1840,8 @@ Module MakeRawList(X:OrderedType)<:S(X).
     rewrite <- rev_cons.
     apply IHo;assumption.
   Qed.
-    
-  Lemma find_decomp_eq : forall e e' ms m m' acc, find_decomp e ms acc = Some(e',m,m') -> 
+
+  Lemma find_decomp_eq : forall e e' ms m m' acc, find_decomp e ms acc = Some(e',m,m') ->
     X.eq e e'.
   Proof.
     intros e e' ms m m' acc.
@@ -1894,11 +1855,11 @@ Module MakeRawList(X:OrderedType)<:S(X).
     assumption.
 
     intros e'0 m m' H.
-    eauto.     
+    eauto.
   Qed.
 
 
-  Function eq_bool (ms1 ms2:t) {struct ms1} : bool := 
+  Function eq_bool (ms1 ms2:t) {struct ms1} : bool :=
     match ms1,ms2 with
       | nil,nil => true
       | e1::ms1,e2::ms2 =>
@@ -1908,7 +1869,7 @@ Module MakeRawList(X:OrderedType)<:S(X).
         end
       | _,_ => false
     end.
-  
+
   Lemma eq_bool_correct : forall m1 m2, eq_bool m1 m2 = true -> eq m1 m2.
   Proof.
     intros m1 m2;functional induction (eq_bool m1 m2);intros Heqb.
@@ -1928,20 +1889,20 @@ Module MakeRawList(X:OrderedType)<:S(X).
   Lemma eq_refl : forall ms, eq ms ms.
   Proof.
     induction ms as [|e ms IH].
-    
-    constructor. 
 
-    change (e :: ms) with (nil ++ e :: ms) at 2. 
+    constructor.
+
+    change (e :: ms) with (nil ++ e :: ms) at 2.
     constructor .
     apply X.eq_refl.
     simpl;assumption.
   Qed.
   Lemma eq_sym : forall ms ms', eq ms ms' -> eq ms' ms.
-  Admitted.     
-    
+  Admitted.
+
   Lemma eq_trans : forall ms1 ms2 ms3, eq ms1 ms2 -> eq ms2 ms3 -> eq ms1 ms3.
   Admitted.
-    
+
 
   Lemma add_morph_eq : forall a a', X.eq a a' -> forall ms ms',  eq ms ms' -> eq (add a ms) (add a' ms'). 
   Proof.
@@ -1978,7 +1939,7 @@ Module MakeRawList(X:OrderedType)<:S(X).
 
   Lemma is_empty_no_mem : forall ms, is_empty ms = true <-> (forall a, mem a ms = false). 
   Proof.
-    
+
     intros ms.
     split.
 
@@ -1995,7 +1956,7 @@ Module MakeRawList(X:OrderedType)<:S(X).
     discriminate.
     elim (XFacts.lt_antirefl l).
   Qed.
-   
+
   Lemma add_is_not_empty : forall a ms, is_empty (add a ms) = false.
   Proof.
     intros a ms.
@@ -2023,12 +1984,12 @@ Module MakeRawList(X:OrderedType)<:S(X).
 
   (* Parameter remove_mem : forall a ms, mem a ms = true -> exists ms', remove a ms = Some ms'. *)
   (* Parameter remove_not_mem : forall a ms, mem a ms = false -> remove a ms = None. *)
- 
+
   Lemma mem_add_comm : forall a b ms, mem a ms = true -> mem a (add b ms) = true.
   Proof.
     intros a b ms;revert b.
     functional induction (mem a ms);try discriminate.
-    
+
     intros b _.
     simpl.
     destruct (XFacts.elim_compare_eq _x).
@@ -2037,7 +1998,7 @@ Module MakeRawList(X:OrderedType)<:S(X).
 
 
     intros b H.
-    
+
     simpl in *.
     destruct (X.compare a e');try tauto;    auto.
   Qed.
